Fix interface.

pulse/lib/pulse/core/PulseCore.IndirectionTheorySep.fst
@@ -1,574 +1,82 @@
 module PulseCore.IndirectionTheorySep
-open PulseCore.IndirectionTheory
-open FStar.FunctionalExtensionality
-module F = FStar.FunctionalExtensionality
-module T = FStar.Tactics
-module RTC = FStar.ReflexiveTransitiveClosure
-module HS = PulseCore.HeapSig
-module E = PulseCore.HeapExtension
-module B = PulseCore.BaseHeapSig
-module IT = PulseCore.IndirectionTheory
-open FStar.Ghost {erased, hide, reveal}
-friend PulseCore.MemoryAlt // FIXME
+module I = PulseCore.IndirectionTheorySepImpl
+open FStar.Ghost
+module PropExt = FStar.PropositionalExtensionality
 
-let address = nat
-let pulse_heap_sig : HS.heap_sig u#3 = PM.sig
-
-[@@erasable]
-noeq type istore_val_ (x: Type u#4) =
-  | None
-  | Inv : x -> istore_val_ x
-  | Pred : x -> istore_val_ x
-
-let istore_val_le #t (x y: istore_val_ t) : prop =
-  match x, y with
-  | None, _ -> True
-  | Inv p, Inv q -> p == q
-  | Pred p, Pred q -> p == q
-  | _ -> False
-
-let map_istore_val #x #y (f: x->y) (v: istore_val_ x) : istore_val_ y =
-  match v with
-  | None -> None
-  | Pred p -> Pred (f p)
-  | Inv p -> Inv (f p)
-
-[@@erasable]
-let invariants (x:Type u#4) : Type u#4 = address ^-> istore_val_ x
-
-let fmap #a #b (f:a -> b) 
-: (invariants a ^-> invariants b)
-= F.on_dom (invariants a) fun x ->
-    F.on_dom address fun a ->
-      map_istore_val f (x a)
-
-let f_ext #t #s (f g: t ^-> s) (h: (x:t -> squash (f x == g x))) : squash (f == g) =
-  introduce forall x. f x == g x with h x;
-  F.extensionality _ _ f g
-
-let fmap_id (a:Type) (x:invariants a)
-: squash (fmap (id #a) == id #(invariants a))
-= f_ext (fmap (id #a)) (id #(invariants a)) fun x ->
-    f_ext (fmap (id #a) x) (id x) fun _ -> ()
-
-
-let fmap_comp (a:Type) (b:Type) (c:Type) (b2c:b -> c) (a2b:a -> b)
-: (squash (compose (fmap b2c) (fmap a2b) ==
-            fmap (compose b2c a2b)))
-= let lhs = compose (fmap b2c) (fmap a2b) in
-  let rhs = fmap (compose b2c a2b) in
-  f_ext lhs rhs fun x -> f_ext (lhs x) (rhs x) fun _ -> ()
-
-noeq
-type rest : Type u#4 = {
-  pulse_heap : pulse_heap_sig.sep.core;
-  saved_credits : erased nat;
-}
-
-let functor_heap : functor u#3 invariants = {
-  fmap = fmap;
-  fmap_id = fmap_id;
-  fmap_comp = fmap_comp;
-  tt = prop;
-  t_bot = False;
-  other = rest;
-}
-
-let istore : Type u#4 = knot_t functor_heap
-
-let preworld = istore & rest
-let world_pred : Type u#4 = preworld ^-> prop
-
-let approx n : (world_pred ^-> world_pred) = approx n
-
-let pulse_heap_le (a b: pulse_heap_sig.sep.core) : prop =
-  exists c. pulse_heap_sig.sep.disjoint a c /\ b == pulse_heap_sig.sep.join a c
-
-let istore_val = istore_val_ world_pred
-
-let read_istore (is: istore) a : istore_val = snd (up is) a
-let read (w: preworld) a = read_istore (fst w) a
-
-let level_istore (is: istore) : nat = level is
-let level_ (w: preworld) : nat = level_istore (fst w)
-
-let approx_def n (p: world_pred) w :
-    Lemma (approx n p w == (if level_ w >= n then False else p w))
-      [SMTPat (approx n p w)] =
-  assert_norm (approx n p w == (if level_ w >= n then False else p w))
-
-let istore_le (x y: istore) : prop =
-  level_istore x == level_istore y /\
-  forall a. istore_val_le (read_istore x a) (read_istore y a)
-
-let world_le (a b: preworld) : prop =
-  let ai, ar = a in
-  let bi, br = b in
-  istore_le ai bi /\
-  pulse_heap_le ar.pulse_heap br.pulse_heap /\
-  ar.saved_credits <= br.saved_credits
-
-let world_pred_affine (p: world_pred) : prop =
-  forall a b. world_le a b /\ p a ==> p b
-
-let age_istore_to (is: istore) (n: nat) : istore =
-  down (n, snd (up is))
-
-let age_to_ (w: preworld) (n: nat) : preworld =
-  (age_istore_to (fst w) n, snd w)
-
-let hereditary (p: world_pred) : prop =
-  forall (w: preworld) (n: nat).
-    n < level_ w /\ p w ==>
-    p (age_to_ w n)
-
-let slprop_ok (p: world_pred) = hereditary p /\ world_pred_affine p
-
-let istore_val_ok (v: istore_val) =
-  match v with
-  | None -> True
-  | Pred p -> slprop_ok p
-  | Inv p -> slprop_ok p
-
-let istore_slprops_ok (is: istore) : prop =
-  forall a. istore_val_ok (read_istore is a)
-
-let world_slprops_ok (w: preworld) : prop =
-  istore_slprops_ok (fst w)
-
-let slprop = p:world_pred { slprop_ok p }
-
-let world = w:preworld { world_slprops_ok w }
-
-let read_age_istore_to (is: istore) n a : Lemma (read_istore (age_istore_to is n) a ==
-    (map_istore_val (approx n) (read_istore is a)))
-    [SMTPat (read_istore (age_istore_to is n) a)] =
-  up_down n (snd (up is))
-
-let read_age_to_ (w: preworld) n a :
-    Lemma (read (age_to_ w n) a == map_istore_val (approx n) (read w a)) =
-  ()
-
-let level_age_istore_to_ is n : Lemma (level_istore (age_istore_to is n) == n) [SMTPat (level_istore (age_istore_to is n))] =
-  up_down n (snd (up is))
-
-let level_age_to_ w n : Lemma (level_ (age_to_ w n) == n) =
-  ()
-
-let age_to (w: world) (n: nat) : world =
-  age_to_ w n
-
-let istore_ext (i1: istore) (i2: istore { level_istore i1 == level_istore i2 })
-    (h: (a:address -> squash (read_istore i1 a == read_istore i2 a))) : squash (i1 == i2) =
-  f_ext (up i1)._2 (up i2)._2 (fun a -> h a);
-  down_up i1;
-  down_up i2
-
-let world_ext (w1: preworld) (w2: preworld { level_ w1 == level_ w2 /\ snd w1 == snd w2 })
-    (h: (a: address -> squash (read w1 a == read w2 a))) : squash (w1 == w2) =
-  istore_ext (fst w1) (fst w2) h
-
-let world_pred_ext (f g: world_pred) (h: (w:preworld -> squash (f w <==> g w))) : squash (f == g) =
-  f_ext f g fun w ->
-    h w;
-    PropositionalExtensionality.apply (f w) (g w)
-
-let approx_approx m n (p: world_pred) : Lemma (approx m (approx n p) == approx (min m n) p) [SMTPat (approx m (approx n p))] =
-  world_pred_ext (approx m (approx n p)) (approx (min m n) p) fun w -> ()
-
-let age_to_age_to (w: preworld) (m n: nat) :
-    Lemma (requires n <= m) (ensures age_to_ (age_to_ w m) n == age_to_ w n)
-      [SMTPat (age_to_ (age_to_ w m) n)] =
-  world_ext (age_to_ (age_to_ w m) n) (age_to_ w n) fun a -> ()
-
-let age_to_rest (w: world) (n: nat) : Lemma ((age_to w n)._2 == w._2) = ()
-
-let level (w: world) : nat = level_ w
-
-let age1_ (w: preworld) : preworld =
-  if level_ w > 0 then age_to_ w (level_ w - 1) else w
-
-let age1 (w: world) : world = age1_ w
-
-let credits (w: world) : GTot nat =
-  w._2.saved_credits
-
-noeq type mem = {
-  invariants: (is:istore { istore_slprops_ok is });
-  pulse_heap : pulse_heap_sig.mem;
-  saved_credits : erased nat;
+noeq type istore = {
+  ist: (is:I.istore { I.istore_slprops_ok is });
+  saved_credits: erased nat;
   freshness_counter: nat;
 }
 
-let core_of (m: mem) : world =
-  (m.invariants, ({ pulse_heap = pulse_heap_sig.sep.core_of m.pulse_heap; saved_credits = m.saved_credits } <: rest))
+noeq type core_istore = {
+  ist: (is:I.istore { I.istore_slprops_ok is });
+  saved_credits: erased nat;
+}
 
-let eq_at (n:nat) (t0 t1:world_pred) =
-  approx n t0 == approx n t1
+// let to_core (w: I.world) : core_istore =
+//   { ist = fst w; saved_credits = (snd w).saved_credits; pulse_mem = (snd w).pulse_heap }
 
-let eq_at_mono (p q: world_pred) m n :
-    Lemma (requires n <= m /\ eq_at m p q) (ensures eq_at n p q)
-      [SMTPat (eq_at m p q); SMTPat (eq_at n p q)] =
-  assert approx n p == approx n (approx m p);
-  assert approx n q == approx n (approx m q)
+let of_core (m: core_mem) : I.world =
+  (m.istore.ist, ({ saved_credits = m.istore.saved_credits; pulse_heap = m.pulse_mem } <: I.rest))
 
-let is_ghost_action = admit ()
-let ghost_action_preorder = admit ()
+let istore_core i = { ist = i.ist; saved_credits = i.saved_credits }
 
-let is_full = admit ()
+let age1 k =
+  { k with istore = { k.istore with ist = I.age1_istore k.istore.ist } }
 
-let interp p w = p w
+let slprop = I.slprop
 
-unfold
-let istore_val_compat (x y: istore_val) =
-  match x, y with
-  | None, _ | _, None -> True
-  | Pred p0, Pred p1 -> p0 == p1
-  | Inv p0, Inv p1 -> p0 == p1
-  | Inv _, Pred _ | Pred _, Inv _ -> False
+let level k = I.level_istore k.istore.ist
 
-let disjoint_istore (is0 is1:istore) =
-  level_istore is0 == level_istore is1 /\
-  (forall a. istore_val_compat (read_istore is0 a) (read_istore is1 a))
+let credits k = k.saved_credits
 
-let disjoint_istore_read is0 is1 a :
-    Lemma (requires disjoint_istore is0 is1)
-      (ensures istore_val_compat (read_istore is0 a) (read_istore is1 a))
-      [SMTPatOr [
-        [SMTPat (disjoint_istore is0 is1); SMTPat (read_istore is0 a)];
-        [SMTPat (disjoint_istore is0 is1); SMTPat (read_istore is1 a)];
-      ]] =
-  ()
+let is_ghost_action_istore = admit ()
 
-let mk_istore n (is: address -> istore_val) : istore =
-  let f' = F.on_dom address is in
-  down (n, f')
+let update_ghost = admit ()
 
-let level_mk_istore n is : Lemma (level_istore (mk_istore n is) == n) [SMTPat (level_istore (mk_istore n is))] =
-  let f' = F.on_dom address is in
-  assert_norm (mk_istore n is == down (n, f'));
-  up_down #_ #functor_heap n f'
+let emp = I.emp
+let pure = I.pure
+let star = I.star
 
-let read_mk_istore n is a :
-    Lemma (read_istore (mk_istore n is) a == map_istore_val (approx n) (is a))
-      [SMTPat (read_istore (mk_istore n is) a)] =
-  let is' = F.on_dom address is in
-  assert_norm (mk_istore n is == down (n, is'));
-  up_down #_ #functor_heap n is';
-  assert_norm (fmap (approx n) is' a == map_istore_val (approx n) (is' a))
+let (exists*) #a f = I.((exists*)) f
 
-let empty_istore n : istore = mk_istore n fun _ -> None
-let empty n : world = (empty_istore n, ({ pulse_heap = pulse_heap_sig.sep.empty; saved_credits = 0 } <: rest))
+let sep_laws = I.sep_laws
 
-let age_to_empty (m n: nat) : Lemma (age_to (empty n) m == empty m) [SMTPat (age_to (empty n) m)] =
-  world_ext (age_to (empty n) m) (empty m) fun a -> read_age_to_ (empty n) m a
+let istore_disjoint i0 i1 = I.disjoint_istore i0.ist i1.ist
 
-let emp : slprop =
-  F.on_dom preworld #(fun _ -> prop) fun w -> True
+let istore_join i0 i1 =
+  { ist = I.join_istore i0.ist i1.ist; saved_credits = i0.saved_credits + i1.saved_credits }
 
-let pure p : slprop = F.on_dom _ fun w -> p
+let istore_join_refl i = I.join_istore_refl i.ist
 
-let join_istore (is0:istore) (is1:istore { disjoint_istore is0 is1 }) : istore =
-  mk_istore (level_istore is0) fun a ->
-    match read_istore is0 a, read_istore is1 a with
-    | None, None -> None
-    | Pred p, _ | _, Pred p -> Pred p
-    | Inv p, _ | _, Inv p -> Inv p
+let interp p =
+  introduce forall (m0 m1:core_mem). p (of_core m0) /\ disjoint m0 m1 ==> p (of_core (join m0 m1)) with
+    introduce _ ==> _ with _.  assert I.world_le (of_core m0) (of_core (join m0 m1));
+  fun m -> p (of_core m)
 
-let read_join_istore (is0:istore) (is1:istore { disjoint_istore is0 is1 }) a :
-  Lemma (read_istore (join_istore is0 is1) a ==
-    (match read_istore is0 a, read_istore is1 a with
-    | None, None -> None
-    | Pred p, _ | _, Pred p -> Pred (approx (level_istore is0) p)
-    | Inv p, _ | _, Inv p -> Inv (approx (level_istore is0) p))) =
-  ()
+let star_equiv p q m = admit ()
 
-let join_istore_commutative (is0:istore) (is1:istore { disjoint_istore is0 is1 }) :
-    Lemma (join_istore is0 is1 == join_istore is1 is0) =
-  istore_ext (join_istore is0 is1) (join_istore is1 is0) fun a -> ()
+let emp_equiv m = ()
 
-let approx_read_istore (is: istore) a :
-    Lemma (map_istore_val (approx (level_istore is)) (read_istore is a) == read_istore is a)
-    [SMTPat (read_istore is a)] =
-  let n, i = up is in down_up is; up_down n i
+let interp_exists p = ()
 
-let join_istore_associative
-    (is0:istore)
-    (is1:istore)
-    (is2:istore { 
-      disjoint_istore is1 is2 /\
-      disjoint_istore is0 (join_istore is1 is2)
-    })
-: Lemma (
-    disjoint_istore is0 is1 /\
-    disjoint_istore (join_istore is0 is1) is2 /\
-    join_istore is0 (join_istore is1 is2) ==
-    join_istore (join_istore is0 is1) is2
-  )
-=
-  istore_ext (join_istore is0 (join_istore is1 is2)) (join_istore (join_istore is0 is1) is2) fun a -> ()
+let interp_pure p m = ()
 
-let istore_le_iff (is1 is2: istore) :
-    Lemma (istore_le is1 is2 <==> exists is3. join_istore is1 is3 == is2) =
-  introduce istore_le is1 is2 ==> exists is3. join_istore is1 is3 == is2 with _.
-    istore_ext (join_istore is1 is2) is2 fun _ -> ()
-
-let disjoint_worlds (w0 w1:preworld)
-: prop 
-= disjoint_istore w0._1 w1._1 /\
-  pulse_heap_sig.sep.disjoint w0._2.pulse_heap w1._2.pulse_heap
-
-let disjoint_world_sym (w0 w1:preworld)
-: Lemma 
-  (ensures disjoint_worlds w0 w1 <==> disjoint_worlds w1 w0)
-= pulse_heap_sig.sep.disjoint_sym w0._2.pulse_heap w1._2.pulse_heap
-
-let join_worlds (w0:preworld) (w1:preworld { disjoint_worlds w0 w1 })
-: preworld
-= (join_istore w0._1 w1._1, ({
-    pulse_heap = pulse_heap_sig.sep.join w0._2.pulse_heap w1._2.pulse_heap;
-    saved_credits = w0._2.saved_credits + w1._2.saved_credits } <: rest))
-
-open FStar.IndefiniteDescription { indefinite_description_ghost }
-
-let world_le_iff (w1 w2: preworld) :
-    Lemma (world_le w1 w2 <==> exists w3. join_worlds w1 w3 == w2) =
-  istore_le_iff (fst w1) (fst w2);
-  introduce world_le w1 w2 ==> exists w3. join_worlds w1 w3 == w2 with _. (
-    assert pulse_heap_le (snd w1).pulse_heap (snd w2).pulse_heap;
-    let ph3 = indefinite_description_ghost _ fun ph3 ->
-      (snd w2).pulse_heap == pulse_heap_sig.sep.join (snd w1).pulse_heap ph3 in
-    let is3 = indefinite_description_ghost _ fun is3 ->
-      fst w2 == join_istore (fst w1) is3 in
-    let sc3: nat = (snd w2).saved_credits - (snd w1).saved_credits in
-    let w3: preworld = (is3, ({ pulse_heap = ph3; saved_credits = sc3 } <: rest)) in
-    assert join_worlds w1 w3 == w2
-  )
-
-let join_worlds_commutative (w0:preworld) (w1:preworld { disjoint_worlds w0 w1 })
-: Lemma (disjoint_worlds w1 w0 /\ join_worlds w0 w1 == join_worlds w1 w0)
-= disjoint_world_sym w0 w1;
-  join_istore_commutative w0._1 w1._1;
-  pulse_heap_sig.sep.join_commutative w0._2.pulse_heap w1._2.pulse_heap
-
-let join_worlds_associative
-    (w0:preworld)
-    (w1:preworld)
-    (w2:preworld { disjoint_worlds w1 w2 /\ disjoint_worlds w0 (join_worlds w1 w2) })
-: Lemma (
-    disjoint_worlds w0 w1 /\
-    disjoint_worlds (join_worlds w0 w1) w2 /\
-    join_worlds w0 (join_worlds w1 w2) ==
-    join_worlds (join_worlds w0 w1) w2
-  )
-= join_istore_associative w0._1 w1._1 w2._1;
-  pulse_heap_sig.sep.join_associative w0._2.pulse_heap w1._2.pulse_heap w2._2.pulse_heap
-
-let age_to_disjoint_worlds (w1 w2: preworld) n :
-    Lemma (requires disjoint_worlds w1 w2)
-      (ensures disjoint_worlds (age_to_ w1 n) (age_to_ w2 n)) =
-  ()
-
-let age_to_join (w1 w2: preworld) n :
-    Lemma (requires disjoint_worlds w1 w2)
-      (ensures disjoint_worlds (age_to_ w1 n) (age_to_ w2 n) /\
-        age_to_ (join_worlds w1 w2) n == join_worlds (age_to_ w1 n) (age_to_ w2 n))
-    [SMTPat (age_to_ (join_worlds w1 w2) n)] =
-  let i1, r1 = w1 in
-  let i2, r1 = w2 in
-  age_to_disjoint_worlds w1 w2 n;
-  istore_ext (age_istore_to (join_istore i1 i2) n) (join_istore (age_istore_to i1 n) (age_istore_to i2 n)) fun a -> ()
-
-let star_ (p1 p2: world_pred) : world_pred =
-  F.on_dom preworld #(fun _ -> prop)
-    fun w -> (exists w1 w2.
-      disjoint_worlds w1 w2 /\ w == join_worlds w1 w2 /\ p1 w1 /\ p2 w2)
-
-[@@"opaque_to_smt"] irreducible
-let indefinite_description_ghost2 (a b: Type) (p: (a -> b -> prop) { exists x y. p x y })
-  : GTot (x: (a&b) { p x._1 x._2 }) =
-  let x = indefinite_description_ghost a fun x -> exists y. p x y in
-  let y = indefinite_description_ghost b fun y -> p x y in
-  (x, y)
-
-let star__commutative (p1 p2:world_pred)
-: Lemma (p1 `star_` p2 == p2 `star_` p1)
-= FStar.Classical.forall_intro_2 disjoint_world_sym;
-  FStar.Classical.forall_intro_2 join_worlds_commutative;
-  world_pred_ext (p1 `star_` p2) (p2 `star_` p1) fun w -> ()
-
-let star__assoc (x y z:world_pred)
-: Lemma (star_ x (star_ y z) == star_ (star_ x y) z)
-=
-  introduce forall x y z w. star_ x (star_ y z) w ==> star_ (star_ x y) z w with introduce _ ==> _ with _. (
-    let (w1, w23) = indefinite_description_ghost2 _ _ fun w1 w23 ->
-      disjoint_worlds w1 w23 /\ w == join_worlds w1 w23 /\ x w1 /\ star_ y z w23 in
-    let (w2, w3) = indefinite_description_ghost2 _ _ fun w2 w3 ->
-      disjoint_worlds w2 w3 /\ w23 == join_worlds w2 w3 /\ y w2 /\ z w3 in
-    join_worlds_associative w1 w2 w3;
-    let w12 = join_worlds w1 w2 in
-    assert star_ x y w12;
-    let w' = join_worlds w12 w3 in
-    assert star_ (star_ x y) z w';
-    assert w == w'
-  );
-  world_pred_ext (star_ x (star_ y z)) (star_ (star_ x y) z) fun w ->
-    star__commutative y z;
-    star__commutative x y;
-    star__commutative x (star_ y z);
-    star__commutative (star_ x y) z;
-    assert star_ x (star_ y z) == star_ (star_ z y) x;
-    assert star_ (star_ x y) z == star_ z (star_ y x)
-
-let star (p1 p2:slprop) : slprop =
-  introduce forall a b. world_le a b /\ star_ p1 p2 a ==> star_ p1 p2 b with introduce _ ==> _ with _. (
-    world_le_iff a b;
-    let c = indefinite_description_ghost _ fun c -> b == join_worlds a c in
-    let (a1, a2) = indefinite_description_ghost2 _ _ fun a1 a2 ->
-      disjoint_worlds a1 a2 /\ a == join_worlds a1 a2 /\ p1 a1 /\ p2 a2 in
-    assert b == join_worlds (join_worlds a1 a2) c;
-    join_worlds_commutative (join_worlds a1 a2) c; 
-    assert b == join_worlds c (join_worlds a1 a2);
-    join_worlds_associative c a1 a2; 
-    assert b == join_worlds (join_worlds c a1) a2;
-    join_worlds_commutative c a1;
-    assert b == join_worlds (join_worlds a1 c) a2;
-    world_le_iff a1 (join_worlds a1 c);
-    assert world_le a1 (join_worlds a1 c);
-    assert p1 (join_worlds a1 c)
-  );
-  star_ p1 p2
-
-let star_commutative (p1 p2:slprop)
-: Lemma (p1 `star` p2 == p2 `star` p1)
-= star__commutative p1 p2
-
-let star_assoc (x y z:slprop)
-: Lemma (star x (star y z) == star (star x y) z)
-= star__assoc x y z
-
-let disjoint_istore_empty is : squash (disjoint_istore (empty_istore (level_istore is)) is) = ()
-
-let join_istore_empty is : squash (join_istore (empty_istore (level_istore is)) is == is) =
-  istore_ext (join_istore (empty_istore (level_istore is)) is) is fun a -> ()
-
-let disjoint_empty w : squash (disjoint_worlds w (empty (level_ w)) /\ disjoint_worlds (empty (level_ w)) w) =
-  pulse_heap_sig.sep.join_empty w._2.pulse_heap;
-  disjoint_world_sym w (empty (level_ w))
-
-let join_empty w : squash (disjoint_worlds (empty (level_ w)) w /\ join_worlds (empty (level_ w)) w == w) =
-  disjoint_empty w;
-  pulse_heap_sig.sep.join_empty w._2.pulse_heap;
-  pulse_heap_sig.sep.join_commutative w._2.pulse_heap pulse_heap_sig.sep.empty;
-  join_istore_empty w._1;
-  world_ext (join_worlds (empty (level_ w)) w) w fun a -> ()
-
-let star_emp (x: slprop) : squash (star x emp == x) =
-  world_pred_ext (star x emp) x fun w ->
-    introduce x w ==> star x emp w with _. (
-      let w2 = empty (level_ w) in
-      join_empty w;
-      join_worlds_commutative w2 w
-    );
-    introduce star x emp w ==> x w with _. (
-      let (w1, w2) = indefinite_description_ghost2 _ _ fun w1 w2 ->
-        disjoint_worlds w1 w2 /\ w == join_worlds w1 w2 /\ x w1 /\ emp w2 in
-      world_le_iff w1 w
-    )
-
-let (exists*) #a f =
-  F.on_dom preworld #(fun _ -> prop) fun w ->
-    exists (x:a). f x w
-
-let sep_laws () =
-  let open PulseCore.Semantics in
-  introduce forall x y. star x y == star y x with star_commutative x y; assert commutative star;
-  introduce forall x y z. star (star x y) z == star x (star y z) with star_assoc x y z; assert associative star;
-  introduce forall x. star x emp == x with star_emp x; assert is_unit emp star
-
-let lift (p: PM.slprop) : slprop =
-  F.on_dom preworld fun w -> pulse_heap_sig.interp p ((snd w).pulse_heap)
-
-let lift_emp_eq () =
-  world_pred_ext (lift PM.emp) emp fun w ->
-    pulse_heap_sig.intro_emp (snd w).pulse_heap
-
-let lift_pure_eq p =
-  world_pred_ext (lift (PM.pure p)) (pure p) fun w ->
-    pulse_heap_sig.pure_interp p (snd w).pulse_heap
-
-// let lift_later_eq #_ = admit ()
-
-let lift_star_eq p q =
-  world_pred_ext (lift (PM.star p q)) (star (lift p) (lift q)) fun w ->
-    pulse_heap_sig.star_equiv p q (snd w).pulse_heap;
-    admit ()
-
+let lift p = I.lift p
+let lift_eq p = ()
+let lift_emp_eq () = I.lift_emp_eq ()
+let lift_pure_eq p = I.lift_pure_eq p
+let lift_star_eq p q = I.lift_star_eq p q
 let lift_exists_eq a f =
-  world_pred_ext (lift (PM.h_exists f)) (exists* x. lift (f x)) fun w ->
-    let f' : a -> GTot pulse_heap_sig.slprop = fun x -> f x in
-    HS.interp_exists f';
-    let m = (snd w).pulse_heap in
-    assert pulse_heap_sig.interp (HS.exists_ f') m <==>
-      (exists x. pulse_heap_sig.interp (f x) m);
-    admit ()
+  I.world_pred_ext (lift PM.(h_exists f)) (exists* x. lift (f x)) fun _ ->
+    I.lift_exists_eq a f
 
-let iref = erased address
+let iref = I.iref
 let deq_iref = fun x y -> reveal x = reveal y
-let lower_inames = admit ()
-let inames_ok = admit ()
-let inames_ok_empty = admit ()
+let lower_inames = admit()
 
-let world_invariant = admit ()
+let istore_inames_ok e m = admit ()
 
-let inv (i:iref) (p:slprop) : slprop =
-  F.on_dom preworld #(fun _ -> prop) fun w ->
-    exists p'.
-      read w i == Inv p' /\
-      eq_at (level_ w) p p'
-
-let later (p: slprop) : slprop =
-  introduce forall (w: preworld) (n: nat).
-      n < level_ w /\ p (age1_ w) ==>
-      p (age1_ (age_to_ w n)) with introduce _ ==> _ with _. (
-    let n' = if n > 0 then n-1 else 0 in
-    assert age_to_ (age1_ w) n' == age_to_ w n'
-  );
-  introduce forall a b. world_le a b /\ p (age1_ a) ==> p (age1_ b) with (
-    world_le_iff a b;
-    world_le_iff (age1_ a) (age1_ b)
-  );
-  F.on_dom preworld fun w -> p (age1_ w)
-
-let timeless (p: slprop) = later p == p
-
-let timeless_lift (p: PM.slprop) : squash (timeless (lift p)) =
-  world_pred_ext (later (lift p)) (lift p) fun w -> ()
-
-let timeless_pure (p: prop) : squash (timeless (pure p)) =
-  world_pred_ext (later (pure p)) (pure p) fun w -> ()
-
-let later_credit n : slprop =
-  F.on_dom preworld #(fun _ -> prop) fun w -> (snd w).saved_credits >= n
-
-let timeless_later_credit n : squash (timeless (later_credit n)) =
-  world_pred_ext (later (later_credit n)) (later_credit n) fun w -> ()
-
-let equiv p q : slprop =
-  F.on_dom preworld #(fun _ -> prop) fun w -> eq_at (level_ w + 1) p q
-
-let eq_at_elim n (p q: world_pred) (w: preworld) :
-    Lemma (requires eq_at n p q /\ level_ w < n) (ensures p w <==> q w) =
-  assert approx n p w == approx n q w
-
-// ----------------
-
-// inv i p  @ w_n  // eq_at n p p'
-
-// i -> Some p' /\ eq_at (n - 1) p p'   @ (agew1 w_n)
-
-// p' (age1 w_n) ///because w_n is an iworld
-
-// have p (age1 w_n) because level (age1 w_n) = n - 1
-
-
+let inames_ok_empty m = admit ()
+let inames_ok_union m = admit ()
