pulse/lib/pulse/core/PulseCore.IndirectionTheorySepImpl.fst
@@ -1,0 +1,577 @@
+module PulseCore.IndirectionTheorySepImpl
+open PulseCore.IndirectionTheory
+open FStar.FunctionalExtensionality
+module F = FStar.FunctionalExtensionality
+module T = FStar.Tactics
+module PM = PulseCore.MemoryAlt
+module RTC = FStar.ReflexiveTransitiveClosure
+module HS = PulseCore.HeapSig
+module E = PulseCore.HeapExtension
+module B = PulseCore.BaseHeapSig
+module IT = PulseCore.IndirectionTheory
+open FStar.Ghost {erased, hide, reveal}
+
+let address = nat
+let pulse_mem : Type u#4 = PM.mem u#0
+let pulse_core_mem : Type u#4 = PM.pulse_heap_sig.sep.core
+let pulse_heap_sig : HS.heap_sig u#3 = PM.pulse_heap_sig
+
+[@@erasable]
+noeq type istore_val_ (x: Type u#4) =
+  | None
+  | Inv : x -> istore_val_ x
+  | Pred : x -> istore_val_ x
+
+let istore_val_le #t (x y: istore_val_ t) : prop =
+  match x, y with
+  | None, _ -> True
+  | Inv p, Inv q -> p == q
+  | Pred p, Pred q -> p == q
+  | _ -> False
+
+let map_istore_val #x #y (f: x->y) (v: istore_val_ x) : istore_val_ y =
+  match v with
+  | None -> None
+  | Pred p -> Pred (f p)
+  | Inv p -> Inv (f p)
+
+[@@erasable]
+let invariants (x:Type u#4) : Type u#4 = address ^-> istore_val_ x
+
+let fmap #a #b (f:a -> b) 
+: (invariants a ^-> invariants b)
+= F.on_dom (invariants a) fun x ->
+    F.on_dom address fun a ->
+      map_istore_val f (x a)
+
+let f_ext #t #s (f g: t ^-> s) (h: (x:t -> squash (f x == g x))) : squash (f == g) =
+  introduce forall x. f x == g x with h x;
+  F.extensionality _ _ f g
+
+let fmap_id (a:Type) (x:invariants a)
+: squash (fmap (id #a) == id #(invariants a))
+= f_ext (fmap (id #a)) (id #(invariants a)) fun x ->
+    f_ext (fmap (id #a) x) (id x) fun _ -> ()
+
+
+let fmap_comp (a:Type) (b:Type) (c:Type) (b2c:b -> c) (a2b:a -> b)
+: (squash (compose (fmap b2c) (fmap a2b) ==
+            fmap (compose b2c a2b)))
+= let lhs = compose (fmap b2c) (fmap a2b) in
+  let rhs = fmap (compose b2c a2b) in
+  f_ext lhs rhs fun x -> f_ext (lhs x) (rhs x) fun _ -> ()
+
+noeq
+type rest : Type u#4 = {
+  pulse_heap : pulse_heap_sig.sep.core;
+  saved_credits : erased nat;
+}
+
+let functor_heap : functor u#3 invariants = {
+  fmap = fmap;
+  fmap_id = fmap_id;
+  fmap_comp = fmap_comp;
+  tt = prop;
+  t_bot = False;
+  other = rest;
+}
+
+let istore : Type u#4 = knot_t functor_heap
+
+let preworld = istore & rest
+let world_pred : Type u#4 = preworld ^-> prop
+
+let approx n : (world_pred ^-> world_pred) = approx n
+
+let pulse_heap_le (a b: pulse_heap_sig.sep.core) : prop =
+  exists c. pulse_heap_sig.sep.disjoint a c /\ b == pulse_heap_sig.sep.join a c
+
+let istore_val = istore_val_ world_pred
+
+let read_istore (is: istore) a : istore_val = snd (up is) a
+let read (w: preworld) a = read_istore (fst w) a
+
+let level_istore (is: istore) : nat = level is
+let level_ (w: preworld) : nat = level_istore (fst w)
+
+let approx_def n (p: world_pred) w :
+    Lemma (approx n p w == (if level_ w >= n then False else p w))
+      [SMTPat (approx n p w)] =
+  assert_norm (approx n p w == (if level_ w >= n then False else p w))
+
+let istore_le (x y: istore) : prop =
+  level_istore x == level_istore y /\
+  forall a. istore_val_le (read_istore x a) (read_istore y a)
+
+let world_le (a b: preworld) : prop =
+  let ai, ar = a in
+  let bi, br = b in
+  istore_le ai bi /\
+  pulse_heap_le ar.pulse_heap br.pulse_heap /\
+  ar.saved_credits <= br.saved_credits
+
+let world_pred_affine (p: world_pred) : prop =
+  forall a b. world_le a b /\ p a ==> p b
+
+let age_istore_to (is: istore) (n: nat) : istore =
+  down (n, snd (up is))
+
+let age_to_ (w: preworld) (n: nat) : preworld =
+  (age_istore_to (fst w) n, snd w)
+
+let hereditary (p: world_pred) : prop =
+  forall (w: preworld) (n: nat).
+    n < level_ w /\ p w ==>
+    p (age_to_ w n)
+
+let slprop_ok (p: world_pred) = hereditary p /\ world_pred_affine p
+
+let istore_val_ok (v: istore_val) =
+  match v with
+  | None -> True
+  | Pred p -> slprop_ok p
+  | Inv p -> slprop_ok p
+
+let istore_slprops_ok (is: istore) : prop =
+  forall a. istore_val_ok (read_istore is a)
+
+let world_slprops_ok (w: preworld) : prop =
+  istore_slprops_ok (fst w)
+
+let slprop = p:world_pred { slprop_ok p }
+
+let world = w:preworld { world_slprops_ok w }
+
+let read_age_istore_to (is: istore) n a : Lemma (read_istore (age_istore_to is n) a ==
+    (map_istore_val (approx n) (read_istore is a)))
+    [SMTPat (read_istore (age_istore_to is n) a)] =
+  up_down n (snd (up is))
+
+let read_age_to_ (w: preworld) n a :
+    Lemma (read (age_to_ w n) a == map_istore_val (approx n) (read w a)) =
+  ()
+
+let level_age_istore_to_ is n : Lemma (level_istore (age_istore_to is n) == n) [SMTPat (level_istore (age_istore_to is n))] =
+  up_down n (snd (up is))
+
+let level_age_to_ w n : Lemma (level_ (age_to_ w n) == n) =
+  ()
+
+let age_to (w: world) (n: nat) : world =
+  age_to_ w n
+
+let istore_ext (i1: istore) (i2: istore { level_istore i1 == level_istore i2 })
+    (h: (a:address -> squash (read_istore i1 a == read_istore i2 a))) : squash (i1 == i2) =
+  f_ext (up i1)._2 (up i2)._2 (fun a -> h a);
+  down_up i1;
+  down_up i2
+
+let world_ext (w1: preworld) (w2: preworld { level_ w1 == level_ w2 /\ snd w1 == snd w2 })
+    (h: (a: address -> squash (read w1 a == read w2 a))) : squash (w1 == w2) =
+  istore_ext (fst w1) (fst w2) h
+
+let world_pred_ext (f g: world_pred) (h: (w:preworld -> squash (f w <==> g w))) : squash (f == g) =
+  f_ext f g fun w ->
+    h w;
+    PropositionalExtensionality.apply (f w) (g w)
+
+let approx_approx m n (p: world_pred) : Lemma (approx m (approx n p) == approx (min m n) p) [SMTPat (approx m (approx n p))] =
+  world_pred_ext (approx m (approx n p)) (approx (min m n) p) fun w -> ()
+
+let age_to_age_to (w: preworld) (m n: nat) :
+    Lemma (requires n <= m) (ensures age_to_ (age_to_ w m) n == age_to_ w n)
+      [SMTPat (age_to_ (age_to_ w m) n)] =
+  world_ext (age_to_ (age_to_ w m) n) (age_to_ w n) fun a -> ()
+
+let age_to_rest (w: world) (n: nat) : Lemma ((age_to w n)._2 == w._2) = ()
+
+let level (w: world) : nat = level_ w
+
+let age1_istore (is: istore) : istore =
+  if level_istore is > 0 then age_istore_to is (level_istore is - 1) else is
+
+let age1_ (w: preworld) : w':preworld { w' == (age1_istore (fst w), snd w) } =
+  if level_ w > 0 then age_to_ w (level_ w - 1) else w
+
+let age1 (w: world) : world = age1_ w
+
+let credits (w: world) : GTot nat =
+  w._2.saved_credits
+
+noeq type mem = {
+  invariants: (is:istore { istore_slprops_ok is });
+  pulse_heap : pulse_heap_sig.mem;
+  saved_credits : erased nat;
+  freshness_counter: nat;
+}
+
+let core_of (m: mem) : world =
+  (m.invariants, ({ pulse_heap = pulse_heap_sig.sep.core_of m.pulse_heap; saved_credits = m.saved_credits } <: rest))
+
+let eq_at (n:nat) (t0 t1:world_pred) =
+  approx n t0 == approx n t1
+
+let eq_at_mono (p q: world_pred) m n :
+    Lemma (requires n <= m /\ eq_at m p q) (ensures eq_at n p q)
+      [SMTPat (eq_at m p q); SMTPat (eq_at n p q)] =
+  assert approx n p == approx n (approx m p);
+  assert approx n q == approx n (approx m q)
+
+let interp p w = p w
+
+unfold
+let istore_val_compat (x y: istore_val) =
+  match x, y with
+  | None, _ | _, None -> True
+  | Pred p0, Pred p1 -> p0 == p1
+  | Inv p0, Inv p1 -> p0 == p1
+  | Inv _, Pred _ | Pred _, Inv _ -> False
+
+let disjoint_istore (is0 is1:istore) =
+  level_istore is0 == level_istore is1 /\
+  (forall a. istore_val_compat (read_istore is0 a) (read_istore is1 a))
+
+let disjoint_istore_read is0 is1 a :
+    Lemma (requires disjoint_istore is0 is1)
+      (ensures istore_val_compat (read_istore is0 a) (read_istore is1 a))
+      [SMTPatOr [
+        [SMTPat (disjoint_istore is0 is1); SMTPat (read_istore is0 a)];
+        [SMTPat (disjoint_istore is0 is1); SMTPat (read_istore is1 a)];
+      ]] =
+  ()
+
+let mk_istore n (is: address -> istore_val) : istore =
+  let f' = F.on_dom address is in
+  down (n, f')
+
+let level_mk_istore n is : Lemma (level_istore (mk_istore n is) == n) [SMTPat (level_istore (mk_istore n is))] =
+  let f' = F.on_dom address is in
+  assert_norm (mk_istore n is == down (n, f'));
+  up_down #_ #functor_heap n f'
+
+let read_mk_istore n is a :
+    Lemma (read_istore (mk_istore n is) a == map_istore_val (approx n) (is a))
+      [SMTPat (read_istore (mk_istore n is) a)] =
+  let is' = F.on_dom address is in
+  assert_norm (mk_istore n is == down (n, is'));
+  up_down #_ #functor_heap n is';
+  assert_norm (fmap (approx n) is' a == map_istore_val (approx n) (is' a))
+
+let empty_istore n : istore = mk_istore n fun _ -> None
+let empty n : world = (empty_istore n, ({ pulse_heap = pulse_heap_sig.sep.empty; saved_credits = 0 } <: rest))
+
+let age_to_empty (m n: nat) : Lemma (age_to (empty n) m == empty m) [SMTPat (age_to (empty n) m)] =
+  world_ext (age_to (empty n) m) (empty m) fun a -> read_age_to_ (empty n) m a
+
+let emp : slprop =
+  F.on_dom preworld #(fun _ -> prop) fun w -> True
+
+let pure p : slprop = F.on_dom _ fun w -> p
+
+let join_istore (is0:istore) (is1:istore { disjoint_istore is0 is1 }) : istore =
+  mk_istore (level_istore is0) fun a ->
+    match read_istore is0 a, read_istore is1 a with
+    | None, None -> None
+    | Pred p, _ | _, Pred p -> Pred p
+    | Inv p, _ | _, Inv p -> Inv p
+
+let read_join_istore (is0:istore) (is1:istore { disjoint_istore is0 is1 }) a :
+  Lemma (read_istore (join_istore is0 is1) a ==
+    (match read_istore is0 a, read_istore is1 a with
+    | None, None -> None
+    | Pred p, _ | _, Pred p -> Pred (approx (level_istore is0) p)
+    | Inv p, _ | _, Inv p -> Inv (approx (level_istore is0) p))) =
+  ()
+
+let join_istore_commutative (is0:istore) (is1:istore { disjoint_istore is0 is1 }) :
+    Lemma (join_istore is0 is1 == join_istore is1 is0) =
+  istore_ext (join_istore is0 is1) (join_istore is1 is0) fun a -> ()
+
+let approx_read_istore (is: istore) a :
+    Lemma (map_istore_val (approx (level_istore is)) (read_istore is a) == read_istore is a)
+    [SMTPat (read_istore is a)] =
+  let n, i = up is in down_up is; up_down n i
+
+let join_istore_refl (is: istore) : Lemma (disjoint_istore is is /\ join_istore is is == is) =
+  istore_ext (join_istore is is) is fun a -> ()
+
+let join_istore_associative
+    (is0:istore)
+    (is1:istore)
+    (is2:istore { 
+      disjoint_istore is1 is2 /\
+      disjoint_istore is0 (join_istore is1 is2)
+    })
+: Lemma (
+    disjoint_istore is0 is1 /\
+    disjoint_istore (join_istore is0 is1) is2 /\
+    join_istore is0 (join_istore is1 is2) ==
+    join_istore (join_istore is0 is1) is2
+  )
+=
+  istore_ext (join_istore is0 (join_istore is1 is2)) (join_istore (join_istore is0 is1) is2) fun a -> ()
+
+let istore_le_iff (is1 is2: istore) :
+    Lemma (istore_le is1 is2 <==> exists is3. join_istore is1 is3 == is2) =
+  introduce istore_le is1 is2 ==> exists is3. join_istore is1 is3 == is2 with _.
+    istore_ext (join_istore is1 is2) is2 fun _ -> ()
+
+let disjoint_worlds (w0 w1:preworld)
+: prop 
+= disjoint_istore w0._1 w1._1 /\
+  pulse_heap_sig.sep.disjoint w0._2.pulse_heap w1._2.pulse_heap
+
+let disjoint_world_sym (w0 w1:preworld)
+: Lemma 
+  (ensures disjoint_worlds w0 w1 <==> disjoint_worlds w1 w0)
+= pulse_heap_sig.sep.disjoint_sym w0._2.pulse_heap w1._2.pulse_heap
+
+let join_worlds (w0:preworld) (w1:preworld { disjoint_worlds w0 w1 })
+: preworld
+= (join_istore w0._1 w1._1, ({
+    pulse_heap = pulse_heap_sig.sep.join w0._2.pulse_heap w1._2.pulse_heap;
+    saved_credits = w0._2.saved_credits + w1._2.saved_credits } <: rest))
+
+open FStar.IndefiniteDescription { indefinite_description_ghost }
+
+let world_le_iff (w1 w2: preworld) :
+    Lemma (world_le w1 w2 <==> exists w3. join_worlds w1 w3 == w2) =
+  istore_le_iff (fst w1) (fst w2);
+  introduce world_le w1 w2 ==> exists w3. join_worlds w1 w3 == w2 with _. (
+    assert pulse_heap_le (snd w1).pulse_heap (snd w2).pulse_heap;
+    let ph3 = indefinite_description_ghost _ fun ph3 ->
+      (snd w2).pulse_heap == pulse_heap_sig.sep.join (snd w1).pulse_heap ph3 in
+    let is3 = indefinite_description_ghost _ fun is3 ->
+      fst w2 == join_istore (fst w1) is3 in
+    let sc3: nat = (snd w2).saved_credits - (snd w1).saved_credits in
+    let w3: preworld = (is3, ({ pulse_heap = ph3; saved_credits = sc3 } <: rest)) in
+    assert join_worlds w1 w3 == w2
+  )
+
+let join_worlds_commutative (w0:preworld) (w1:preworld { disjoint_worlds w0 w1 })
+: Lemma (disjoint_worlds w1 w0 /\ join_worlds w0 w1 == join_worlds w1 w0)
+= disjoint_world_sym w0 w1;
+  join_istore_commutative w0._1 w1._1;
+  pulse_heap_sig.sep.join_commutative w0._2.pulse_heap w1._2.pulse_heap
+
+let join_worlds_associative
+    (w0:preworld)
+    (w1:preworld)
+    (w2:preworld { disjoint_worlds w1 w2 /\ disjoint_worlds w0 (join_worlds w1 w2) })
+: Lemma (
+    disjoint_worlds w0 w1 /\
+    disjoint_worlds (join_worlds w0 w1) w2 /\
+    join_worlds w0 (join_worlds w1 w2) ==
+    join_worlds (join_worlds w0 w1) w2
+  )
+= join_istore_associative w0._1 w1._1 w2._1;
+  pulse_heap_sig.sep.join_associative w0._2.pulse_heap w1._2.pulse_heap w2._2.pulse_heap
+
+let age_to_disjoint_worlds (w1 w2: preworld) n :
+    Lemma (requires disjoint_worlds w1 w2)
+      (ensures disjoint_worlds (age_to_ w1 n) (age_to_ w2 n)) =
+  ()
+
+let age_to_join (w1 w2: preworld) n :
+    Lemma (requires disjoint_worlds w1 w2)
+      (ensures disjoint_worlds (age_to_ w1 n) (age_to_ w2 n) /\
+        age_to_ (join_worlds w1 w2) n == join_worlds (age_to_ w1 n) (age_to_ w2 n))
+    [SMTPat (age_to_ (join_worlds w1 w2) n)] =
+  let i1, r1 = w1 in
+  let i2, r1 = w2 in
+  age_to_disjoint_worlds w1 w2 n;
+  istore_ext (age_istore_to (join_istore i1 i2) n) (join_istore (age_istore_to i1 n) (age_istore_to i2 n)) fun a -> ()
+
+let star_ (p1 p2: world_pred) : world_pred =
+  F.on_dom preworld #(fun _ -> prop)
+    fun w -> (exists w1 w2.
+      disjoint_worlds w1 w2 /\ w == join_worlds w1 w2 /\ p1 w1 /\ p2 w2)
+
+[@@"opaque_to_smt"] irreducible
+let indefinite_description_ghost2 (a b: Type) (p: (a -> b -> prop) { exists x y. p x y })
+  : GTot (x: (a&b) { p x._1 x._2 }) =
+  let x = indefinite_description_ghost a fun x -> exists y. p x y in
+  let y = indefinite_description_ghost b fun y -> p x y in
+  (x, y)
+
+let star__commutative (p1 p2:world_pred)
+: Lemma (p1 `star_` p2 == p2 `star_` p1)
+= FStar.Classical.forall_intro_2 disjoint_world_sym;
+  FStar.Classical.forall_intro_2 join_worlds_commutative;
+  world_pred_ext (p1 `star_` p2) (p2 `star_` p1) fun w -> ()
+
+let star__assoc (x y z:world_pred)
+: Lemma (star_ x (star_ y z) == star_ (star_ x y) z)
+=
+  introduce forall x y z w. star_ x (star_ y z) w ==> star_ (star_ x y) z w with introduce _ ==> _ with _. (
+    let (w1, w23) = indefinite_description_ghost2 _ _ fun w1 w23 ->
+      disjoint_worlds w1 w23 /\ w == join_worlds w1 w23 /\ x w1 /\ star_ y z w23 in
+    let (w2, w3) = indefinite_description_ghost2 _ _ fun w2 w3 ->
+      disjoint_worlds w2 w3 /\ w23 == join_worlds w2 w3 /\ y w2 /\ z w3 in
+    join_worlds_associative w1 w2 w3;
+    let w12 = join_worlds w1 w2 in
+    assert star_ x y w12;
+    let w' = join_worlds w12 w3 in
+    assert star_ (star_ x y) z w';
+    assert w == w'
+  );
+  world_pred_ext (star_ x (star_ y z)) (star_ (star_ x y) z) fun w ->
+    star__commutative y z;
+    star__commutative x y;
+    star__commutative x (star_ y z);
+    star__commutative (star_ x y) z;
+    assert star_ x (star_ y z) == star_ (star_ z y) x;
+    assert star_ (star_ x y) z == star_ z (star_ y x)
+
+let star (p1 p2:slprop) : slprop =
+  introduce forall a b. world_le a b /\ star_ p1 p2 a ==> star_ p1 p2 b with introduce _ ==> _ with _. (
+    world_le_iff a b;
+    let c = indefinite_description_ghost _ fun c -> b == join_worlds a c in
+    let (a1, a2) = indefinite_description_ghost2 _ _ fun a1 a2 ->
+      disjoint_worlds a1 a2 /\ a == join_worlds a1 a2 /\ p1 a1 /\ p2 a2 in
+    assert b == join_worlds (join_worlds a1 a2) c;
+    join_worlds_commutative (join_worlds a1 a2) c; 
+    assert b == join_worlds c (join_worlds a1 a2);
+    join_worlds_associative c a1 a2; 
+    assert b == join_worlds (join_worlds c a1) a2;
+    join_worlds_commutative c a1;
+    assert b == join_worlds (join_worlds a1 c) a2;
+    world_le_iff a1 (join_worlds a1 c);
+    assert world_le a1 (join_worlds a1 c);
+    assert p1 (join_worlds a1 c)
+  );
+  star_ p1 p2
+
+let star_commutative (p1 p2:slprop)
+: Lemma (p1 `star` p2 == p2 `star` p1)
+= star__commutative p1 p2
+
+let star_assoc (x y z:slprop)
+: Lemma (star x (star y z) == star (star x y) z)
+= star__assoc x y z
+
+let disjoint_istore_empty is : squash (disjoint_istore (empty_istore (level_istore is)) is) = ()
+
+let join_istore_empty is : squash (join_istore (empty_istore (level_istore is)) is == is) =
+  istore_ext (join_istore (empty_istore (level_istore is)) is) is fun a -> ()
+
+let disjoint_empty w : squash (disjoint_worlds w (empty (level_ w)) /\ disjoint_worlds (empty (level_ w)) w) =
+  pulse_heap_sig.sep.join_empty w._2.pulse_heap;
+  disjoint_world_sym w (empty (level_ w))
+
+let join_empty w : squash (disjoint_worlds (empty (level_ w)) w /\ join_worlds (empty (level_ w)) w == w) =
+  disjoint_empty w;
+  pulse_heap_sig.sep.join_empty w._2.pulse_heap;
+  pulse_heap_sig.sep.join_commutative w._2.pulse_heap pulse_heap_sig.sep.empty;
+  join_istore_empty w._1;
+  world_ext (join_worlds (empty (level_ w)) w) w fun a -> ()
+
+let star_emp (x: slprop) : squash (star x emp == x) =
+  world_pred_ext (star x emp) x fun w ->
+    introduce x w ==> star x emp w with _. (
+      let w2 = empty (level_ w) in
+      join_empty w;
+      join_worlds_commutative w2 w
+    );
+    introduce star x emp w ==> x w with _. (
+      let (w1, w2) = indefinite_description_ghost2 _ _ fun w1 w2 ->
+        disjoint_worlds w1 w2 /\ w == join_worlds w1 w2 /\ x w1 /\ emp w2 in
+      world_le_iff w1 w
+    )
+
+let (exists*) #a f =
+  F.on_dom preworld #(fun _ -> prop) fun w ->
+    exists (x:a). f x w
+
+let sep_laws (_:unit) : squash (
+  PulseCore.Semantics.(
+    associative star /\
+    commutative star /\
+    is_unit emp star
+  )
+) =
+  let open PulseCore.Semantics in
+  introduce forall x y. star x y == star y x with star_commutative x y; assert commutative star;
+  introduce forall x y z. star (star x y) z == star x (star y z) with star_assoc x y z; assert associative star;
+  introduce forall x. star x emp == x with star_emp x; assert is_unit emp star
+
+let lift (p: PM.slprop) : slprop =
+  F.on_dom preworld fun w -> pulse_heap_sig.interp p ((snd w).pulse_heap)
+
+let lift_emp_eq () =
+  world_pred_ext (lift PM.emp) emp fun w ->
+    pulse_heap_sig.intro_emp (snd w).pulse_heap
+
+let lift_pure_eq p =
+  world_pred_ext (lift (PM.pure p)) (pure p) fun w ->
+    pulse_heap_sig.pure_interp p (snd w).pulse_heap
+
+// let lift_later_eq #_ = admit ()
+
+let lift_star_eq p q =
+  world_pred_ext (lift (PM.star p q)) (star (lift p) (lift q)) fun w ->
+    pulse_heap_sig.star_equiv p q (snd w).pulse_heap;
+    admit ()
+
+let lift_exists_eq a f =
+  world_pred_ext (lift (PM.h_exists f)) (exists* x. lift (f x)) fun w ->
+    let f' : a -> GTot pulse_heap_sig.slprop = fun x -> f x in
+    HS.interp_exists f';
+    let m = (snd w).pulse_heap in
+    assert pulse_heap_sig.interp (HS.exists_ f') m <==>
+      (exists x. pulse_heap_sig.interp (f x) m);
+    admit ()
+
+let iref = erased address
+
+let inv (i:iref) (p:slprop) : slprop =
+  F.on_dom preworld #(fun _ -> prop) fun w ->
+    exists p'.
+      read w i == Inv p' /\
+      eq_at (level_ w) p p'
+
+let later (p: slprop) : slprop =
+  introduce forall (w: preworld) (n: nat).
+      n < level_ w /\ p (age1_ w) ==>
+      p (age1_ (age_to_ w n)) with introduce _ ==> _ with _. (
+    let n' = if n > 0 then n-1 else 0 in
+    assert age_to_ (age1_ w) n' == age_to_ w n'
+  );
+  introduce forall a b. world_le a b /\ p (age1_ a) ==> p (age1_ b) with (
+    world_le_iff a b;
+    world_le_iff (age1_ a) (age1_ b)
+  );
+  F.on_dom preworld fun w -> p (age1_ w)
+
+let timeless (p: slprop) = later p == p
+
+let timeless_lift (p: PM.slprop) : squash (timeless (lift p)) =
+  world_pred_ext (later (lift p)) (lift p) fun w -> ()
+
+let timeless_pure (p: prop) : squash (timeless (pure p)) =
+  world_pred_ext (later (pure p)) (pure p) fun w -> ()
+
+let later_credit n : slprop =
+  F.on_dom preworld #(fun _ -> prop) fun w -> (snd w).saved_credits >= n
+
+let timeless_later_credit n : squash (timeless (later_credit n)) =
+  world_pred_ext (later (later_credit n)) (later_credit n) fun w -> ()
+
+let equiv p q : slprop =
+  F.on_dom preworld #(fun _ -> prop) fun w -> eq_at (level_ w + 1) p q
+
+let eq_at_elim n (p q: world_pred) (w: preworld) :
+    Lemma (requires eq_at n p q /\ level_ w < n) (ensures p w <==> q w) =
+  assert approx n p w == approx n q w
+
+// ----------------
+
+// inv i p  @ w_n  // eq_at n p p'
+
+// i -> Some p' /\ eq_at (n - 1) p p'   @ (agew1 w_n)
+
+// p' (age1 w_n) ///because w_n is an iworld
+
+// have p (age1 w_n) because level (age1 w_n) = n - 1
+
+
